Covalence/HasTySubterm.lean
@@ -1,0 +1,549 @@
+import Covalence.HasTy
+import Mathlib.Data.Set.Lattice.Image
+
+def Tm.BSubst.cvar (σ : Tm.BSubst) (x : ℕ) : Tm.BSubst
+  | 0 => .fv x
+  | x + 1 => σ.get x
+
+@[simp]
+theorem Tm.BSubst.cvar_get_zero (σ : Tm.BSubst) (x : ℕ) : (σ.cvar x).get 0 = .fv x := rfl
+
+@[simp]
+theorem Tm.BSubst.cvar_get_succ (σ : Tm.BSubst) (x i : ℕ) : (σ.cvar x).get (i + 1) = σ.get i := rfl
+
+theorem Tm.BSubst.cvar_mul_lift (σ τ : Tm.BSubst) (x : ℕ) : (σ.cvar x) * ↑s τ = (σ * τ).cvar x := by
+  ext i
+  cases i with
+  | zero => rfl
+  | succ i =>
+    simp only [get_mul, get_succ_lift, ← bsubst_wkIn, cvar_get_succ]
+    rfl
+
+def Ctx.closeSubtermsOver (Γ : Ctx) (σ : Tm.BSubst) : Tm → Set Tm
+  | .eqn A a b =>
+    { .bsubst σ (.eqn A a b) }
+    ∪ Γ.closeSubtermsOver σ A ∪ Γ.closeSubtermsOver σ a ∪ Γ.closeSubtermsOver σ b
+  | .pi A B =>
+    { .bsubst σ (.pi A B) }
+    ∪ Γ.closeSubtermsOver σ A ∪ ⋃x ∉ Γ.dv, (Γ.cons x A).closeSubtermsOver (σ.cvar x) B
+  | .abs A B b =>
+    { .bsubst σ (.abs A B b) }
+    ∪ Γ.closeSubtermsOver σ A
+    ∪ (⋃x ∉ Γ.dv, (Γ.cons x A).closeSubtermsOver (σ.cvar x) B)
+    ∪ (⋃x ∉ Γ.dv, (Γ.cons x A).closeSubtermsOver (σ.cvar x) b)
+  | .app A B f a =>
+    { .bsubst σ (.app A B f a) }
+    ∪ Γ.closeSubtermsOver σ A
+    ∪ (⋃x ∉ Γ.dv, (Γ.cons x A).closeSubtermsOver (σ.cvar x) B)
+    ∪ Γ.closeSubtermsOver σ f
+    ∪ Γ.closeSubtermsOver σ a
+  | .sigma A B =>
+    { .bsubst σ (.sigma A B) }
+    ∪ Γ.closeSubtermsOver σ A ∪
+    (⋃x ∉ Γ.dv, (Γ.cons x A).closeSubtermsOver (σ.cvar x) B)
+  | .pair A B a b =>
+    { .bsubst σ (.pair A B a b) }
+    ∪ Γ.closeSubtermsOver σ A
+    ∪ (⋃x ∉ Γ.dv, (Γ.cons x A).closeSubtermsOver (σ.cvar x) B)
+    ∪ Γ.closeSubtermsOver σ a
+    ∪ Γ.closeSubtermsOver σ b
+  | .fst A B a =>
+    { .bsubst σ (.fst A B a) }
+    ∪ Γ.closeSubtermsOver σ A
+    ∪ (⋃x ∉ Γ.dv, (Γ.cons x A).closeSubtermsOver (σ.cvar x) B)
+    ∪ Γ.closeSubtermsOver σ a
+  | .snd A B a =>
+    { .bsubst σ (.snd A B a) }
+    ∪ Γ.closeSubtermsOver σ A
+    ∪ (⋃x ∉ Γ.dv, (Γ.cons x A).closeSubtermsOver (σ.cvar x) B)
+    ∪ Γ.closeSubtermsOver σ a
+  | .dite φ A a b =>
+    { .bsubst σ (.dite φ A a b) }
+    ∪ Γ.closeSubtermsOver σ φ
+    ∪ Γ.closeSubtermsOver σ A
+    ∪ Γ.closeSubtermsOver σ A
+    ∪ (⋃x ∉ Γ.dv, (Γ.cons x φ).closeSubtermsOver σ a)
+    ∪ (⋃x ∉ Γ.dv, (Γ.cons x φ.not).closeSubtermsOver σ b)
+  | .trunc A =>
+    { .bsubst σ (.trunc A) }
+    ∪ Γ.closeSubtermsOver σ A
+  | .choose A φ =>
+    { .bsubst σ (.choose A φ) }
+    ∪ Γ.closeSubtermsOver σ A
+    ∪ (⋃x ∉ Γ.dv, (Γ.cons x A).closeSubtermsOver (σ.cvar x) φ)
+  | .natrec C n z s =>
+    { .bsubst σ (.natrec C n z s) }
+    ∪ (⋃x ∉ Γ.dv, (Γ.cons x .nats).closeSubtermsOver (σ.cvar x) C)
+    ∪ Γ.closeSubtermsOver σ n
+    ∪ Γ.closeSubtermsOver σ z
+    ∪ (⋃x ∉ Γ.dv, (Γ.cons x .nats).closeSubtermsOver (σ.cvar x) s)
+  | .let₁ A a b =>
+    { .bsubst σ (.let₁ A a b) }
+    ∪ Γ.closeSubtermsOver σ A
+    ∪ Γ.closeSubtermsOver σ a
+    ∪ ⋃x ∉ Γ.dv, (Γ.cons x A).closeSubtermsOver (σ.cvar x) b
+  | .bv i => { σ.get i }
+  | a => { a }
+
+theorem Ctx.closeSubtermsOver_dvs (Γ Δ : Ctx) (h : Γ.dv = Δ.dv)
+  : Γ.closeSubtermsOver = Δ.closeSubtermsOver := by
+  funext σ a
+  induction a generalizing Γ Δ σ with
+  | _ =>
+    simp only [closeSubtermsOver] <;>
+    congr <;> first
+    | (apply_assumption; exact h)
+    | (
+      rw [h]
+      apply Set.iUnion₂_congr
+      intro x hx
+      apply_assumption
+      simp [Ctx.dv, h]
+    )
+
+theorem Ctx.closeSubtermsOver_dvs_left_cons
+  (Γ : Ctx) (x : ℕ) (A B : Tm) (σ τ : Tm.BSubst) (a b : Tm)
+  (h : (Γ.cons x A).closeSubtermsOver σ a = (Γ.cons x A).closeSubtermsOver τ b)
+  : (Γ.cons x A).closeSubtermsOver σ a = (Γ.cons x B).closeSubtermsOver τ b := by
+  rw [h, closeSubtermsOver_dvs]; simp only [Ctx.dv]
+
+theorem Ctx.closeSubtermsOver_dvs_right_cons
+  (Γ : Ctx) (x : ℕ) (A B : Tm) (σ τ : Tm.BSubst) (a b : Tm)
+  (h : (Γ.cons x B).closeSubtermsOver σ a = (Γ.cons x B).closeSubtermsOver τ b)
+  : (Γ.cons x A).closeSubtermsOver σ a = (Γ.cons x B).closeSubtermsOver τ b := by
+  rw [<-h, closeSubtermsOver_dvs]; simp only [Ctx.dv]
+
+inductive Tm.IsVar : Tm → Prop
+  | bv (i : ℕ) : IsVar (.bv i)
+  | fv (x : ℕ) : IsVar (.fv x)
+
+def Tm.BSubst.Vars (σ : Tm.BSubst) : Prop := ∀ (i : ℕ), (σ.get i).IsVar
+
+theorem Tm.BSubst.Vars.one : (1 : BSubst).Vars := fun i => .bv i
+
+theorem Tm.IsVar.lift {t : Tm} (h : t.IsVar) : (↑0 t).IsVar := by cases h <;> constructor
+
+theorem Tm.BSubst.Vars.lift {σ : Tm.BSubst} (hσ : σ.Vars) : (↑s σ).Vars
+  := fun | 0 => .bv 0 | i + 1 => (hσ i).lift
+
+theorem Tm.BSubst.Vars.cvar {σ : Tm.BSubst} (hσ : σ.Vars) (x : ℕ) : (σ.cvar x).Vars
+  := fun | 0 => .fv x | i + 1 => hσ i
+
+def Ctx.closeSubtermsOver_bsubst (Γ : Ctx) {σ τ : Tm.BSubst} (hτ : τ.Vars) (a : Tm)
+  : Γ.closeSubtermsOver σ (a.bsubst τ) = Γ.closeSubtermsOver (σ * τ) a
+  := by induction a generalizing σ τ Γ with
+  | bv i =>
+    simp only [Tm.bsubst, closeSubtermsOver, Tm.BSubst.get_mul]
+    have ht := hτ i
+    generalize τ.get i = t at *
+    cases ht <;> simp only [closeSubtermsOver, Tm.bsubst]
+  | _ =>
+    simp only [closeSubtermsOver, Tm.bsubst, Tm.bsubst_bsubst, Tm.BSubst.lift_mul, *]
+    <;> congr
+    <;> {
+      apply Set.iUnion₂_congr
+      intro x hx
+      apply Ctx.closeSubtermsOver_dvs_left_cons
+      simp only [<-Tm.BSubst.cvar_mul_lift σ τ, hτ.lift, *]
+    }
+
+theorem Ctx.closeSubtermsOver_cvar1 (Γ : Ctx) (x : ℕ) (a : Tm)
+  : Γ.closeSubtermsOver ((1 : Tm.BSubst).cvar x) a = Γ.closeSubtermsOver 1 (a.bs0 (.fv x))
+  := by
+  rw [Tm.bs0, closeSubtermsOver_bsubst]
+  · apply congrFun; apply congrArg; ext i; cases i <;> rfl
+  · intro i; cases i <;> constructor
+
+@[simp]
+theorem Ctx.closeSubtermsOver_fv (Γ : Ctx) (σ : Tm.BSubst) (x : ℕ)
+  : Γ.closeSubtermsOver σ (.fv x) = { .fv x }
+  := rfl
+
+@[simp]
+theorem Ctx.closeSubtermsOver1_bv (Γ : Ctx) (i : ℕ)
+  : Γ.closeSubtermsOver 1 (.bv i) = { .bv i }
+  := rfl
+
+@[simp]
+theorem Ctx.closeSubtermsOver_univ (Γ : Ctx) (σ : Tm.BSubst) (ℓ : ℕ)
+  : Γ.closeSubtermsOver σ (.univ ℓ) = { .univ ℓ }
+  := rfl
+
+@[simp]
+theorem Ctx.closeSubtermsOver_unit (Γ : Ctx) (σ : Tm.BSubst) (ℓ : ℕ)
+  : Γ.closeSubtermsOver σ (.unit ℓ) = { .unit ℓ }
+  := rfl
+
+@[simp]
+theorem Ctx.closeSubtermsOver_nil (Γ : Ctx) (σ : Tm.BSubst) (ℓ : ℕ)
+  : Γ.closeSubtermsOver σ (.nil ℓ) = { .nil ℓ }
+  := rfl
+
+@[simp]
+theorem Ctx.closeSubtermsOver_empty (Γ : Ctx) (σ : Tm.BSubst) (ℓ : ℕ)
+  : Γ.closeSubtermsOver σ (.empty ℓ) = { .empty ℓ }
+  := rfl
+
+@[simp]
+theorem Ctx.closeSubtermsOver1_eqn (Γ : Ctx) (A a b : Tm)
+  : Γ.closeSubtermsOver 1 (.eqn A a b) = { .eqn A a b }
+    ∪ Γ.closeSubtermsOver 1 A
+    ∪ Γ.closeSubtermsOver 1 a
+    ∪ Γ.closeSubtermsOver 1 b
+  := by simp [closeSubtermsOver]
+
+@[simp]
+theorem Ctx.closeSubtermsOver1_pi (Γ : Ctx) (A B : Tm)
+  : Γ.closeSubtermsOver 1 (.pi A B) = { .pi A B }
+    ∪ Γ.closeSubtermsOver 1 A
+    ∪ ⋃x ∉ Γ.dv, (Γ.cons x A).closeSubtermsOver 1 (B.bs0 (.fv x))
+  := by simp [closeSubtermsOver, Ctx.closeSubtermsOver_cvar1]
+
+@[simp]
+theorem Ctx.closeSubtermsOver1_abs (Γ : Ctx) (A B b : Tm)
+  : Γ.closeSubtermsOver 1 (.abs A B b) = { .abs A B b }
+    ∪ Γ.closeSubtermsOver 1 A
+    ∪ (⋃x ∉ Γ.dv, (Γ.cons x A).closeSubtermsOver 1 (B.bs0 (.fv x)))
+    ∪ (⋃x ∉ Γ.dv, (Γ.cons x A).closeSubtermsOver 1 (b.bs0 (.fv x)))
+  := by simp [closeSubtermsOver, Ctx.closeSubtermsOver_cvar1]
+
+@[simp]
+theorem Ctx.closeSubtermsOver1_app (Γ : Ctx) (A B f a : Tm)
+  : Γ.closeSubtermsOver 1 (.app A B f a) = { .app A B f a }
+    ∪ Γ.closeSubtermsOver 1 A
+    ∪ (⋃x ∉ Γ.dv, (Γ.cons x A).closeSubtermsOver 1 (B.bs0 (.fv x)))
+    ∪ Γ.closeSubtermsOver 1 f
+    ∪ Γ.closeSubtermsOver 1 a
+  := by simp [closeSubtermsOver, Ctx.closeSubtermsOver_cvar1]
+
+@[simp]
+theorem Ctx.closeSubtermsOver1_sigma (Γ : Ctx) (A B : Tm)
+  : Γ.closeSubtermsOver 1 (.sigma A B) = { .sigma A B }
+    ∪ Γ.closeSubtermsOver 1 A
+    ∪ (⋃x ∉ Γ.dv, (Γ.cons x A).closeSubtermsOver 1 (B.bs0 (.fv x)))
+  := by simp [closeSubtermsOver, Ctx.closeSubtermsOver_cvar1]
+
+@[simp]
+theorem Ctx.closeSubtermsOver1_pair (Γ : Ctx) (A B a b : Tm)
+  : Γ.closeSubtermsOver 1 (.pair A B a b) = { .pair A B a b }
+    ∪ Γ.closeSubtermsOver 1 A
+    ∪ (⋃x ∉ Γ.dv, (Γ.cons x A).closeSubtermsOver 1 (B.bs0 (.fv x)))
+    ∪ Γ.closeSubtermsOver 1 a
+    ∪ Γ.closeSubtermsOver 1 b
+  := by simp [closeSubtermsOver, Ctx.closeSubtermsOver_cvar1]
+
+@[simp]
+theorem Ctx.closeSubtermsOver1_fst (Γ : Ctx) (A B a : Tm)
+  : Γ.closeSubtermsOver 1 (.fst A B a) = { .fst A B a }
+    ∪ Γ.closeSubtermsOver 1 A
+    ∪ (⋃x ∉ Γ.dv, (Γ.cons x A).closeSubtermsOver 1 (B.bs0 (.fv x)))
+    ∪ Γ.closeSubtermsOver 1 a
+  := by simp [closeSubtermsOver, Ctx.closeSubtermsOver_cvar1]
+
+@[simp]
+theorem Ctx.closeSubtermsOver1_snd (Γ : Ctx) (A B a : Tm)
+  : Γ.closeSubtermsOver 1 (.snd A B a) = { .snd A B a }
+    ∪ Γ.closeSubtermsOver 1 A
+    ∪ (⋃x ∉ Γ.dv, (Γ.cons x A).closeSubtermsOver 1 (B.bs0 (.fv x)))
+    ∪ Γ.closeSubtermsOver 1 a
+  := by simp [closeSubtermsOver, Ctx.closeSubtermsOver_cvar1]
+
+@[simp]
+theorem Ctx.closeSubtermsOver1_dite (Γ : Ctx) (φ A a b : Tm)
+  : Γ.closeSubtermsOver 1 (.dite φ A a b) = { .dite φ A a b }
+    ∪ Γ.closeSubtermsOver 1 φ
+    ∪ Γ.closeSubtermsOver 1 A
+    ∪ Γ.closeSubtermsOver 1 A
+    ∪ (⋃x ∉ Γ.dv, (Γ.cons x φ).closeSubtermsOver 1 a)
+    ∪ (⋃x ∉ Γ.dv, (Γ.cons x φ.not).closeSubtermsOver 1 b)
+  := by simp [closeSubtermsOver]
+
+@[simp]
+theorem Ctx.closeSubtermsOver1_trunc (Γ : Ctx) (A : Tm)
+  : Γ.closeSubtermsOver 1 (.trunc A) = { .trunc A }
+    ∪ Γ.closeSubtermsOver 1 A
+  := by simp [closeSubtermsOver]
+
+@[simp]
+theorem Ctx.closeSubtermsOver1_choose (Γ : Ctx) (A φ : Tm)
+  : Γ.closeSubtermsOver 1 (.choose A φ) = { .choose A φ }
+    ∪ Γ.closeSubtermsOver 1 A
+    ∪ (⋃x ∉ Γ.dv, (Γ.cons x A).closeSubtermsOver 1 (φ.bs0 (.fv x)))
+  := by simp [closeSubtermsOver, Ctx.closeSubtermsOver_cvar1]
+
+@[simp]
+theorem Ctx.closeSubtermsOver_nats (Γ : Ctx) (σ : Tm.BSubst)
+  : Γ.closeSubtermsOver σ .nats = { .nats }
+  := rfl
+
+@[simp]
+theorem Ctx.closeSubtermsOver_zero (Γ : Ctx) (σ : Tm.BSubst)
+  : Γ.closeSubtermsOver σ .zero = { .zero }
+  := rfl
+
+@[simp]
+theorem Ctx.closeSubtermsOver_succ (Γ : Ctx) (σ : Tm.BSubst)
+  : Γ.closeSubtermsOver σ .succ = { .succ }
+  := rfl
+
+@[simp]
+theorem Ctx.closeSubtermsOver_natrec (Γ : Ctx) (C n z s : Tm)
+  : Γ.closeSubtermsOver 1 (.natrec C n z s) = { .natrec C n z s }
+    ∪ (⋃x ∉ Γ.dv, (Γ.cons x .nats).closeSubtermsOver 1 (C.bs0 (.fv x)))
+    ∪ Γ.closeSubtermsOver 1 n
+    ∪ Γ.closeSubtermsOver 1 z
+    ∪ (⋃x ∉ Γ.dv, (Γ.cons x .nats).closeSubtermsOver 1 (s.bs0 (.fv x)))
+  := by simp [closeSubtermsOver, Ctx.closeSubtermsOver_cvar1]
+
+@[simp]
+theorem Ctx.closeSubtermsOver_let₁ (Γ : Ctx) (A a b : Tm)
+  : Γ.closeSubtermsOver 1 (.let₁ A a b) = { .let₁ A a b }
+    ∪ Γ.closeSubtermsOver 1 A
+    ∪ Γ.closeSubtermsOver 1 a
+    ∪ ⋃x ∉ Γ.dv, (Γ.cons x A).closeSubtermsOver 1 (b.bs0 (.fv x))
+  := by simp [closeSubtermsOver, Ctx.closeSubtermsOver_cvar1]
+
+@[simp]
+theorem Ctx.closeSubtermsOver_invalid (Γ : Ctx) (σ : Tm.BSubst)
+  : Γ.closeSubtermsOver σ .invalid = { .invalid }
+  := rfl
+
+theorem Ctx.closeSubtermsOver_anti (Γ Δ : Ctx) (σ : Tm.BSubst) (a : Tm) (h : Γ.dv ⊆ Δ.dv)
+  : Δ.closeSubtermsOver σ a ⊆ Γ.closeSubtermsOver σ a := by
+  induction a generalizing Γ Δ σ <;> simp only [closeSubtermsOver, Set.Subset.refl]
+  <;> (repeat first | apply Set.union_subset_union)
+  <;> (try simp only [Set.Subset.refl, *])
+  <;> {
+    apply Set.iUnion_mono
+    intro x
+    simp only [Set.iUnion_subset_iff]
+    intro hx
+    have hx' : x ∉ Γ.dv := Set.notMem_subset h hx
+    simp only [hx', not_false_eq_true, Set.iUnion_true]
+    apply_assumption
+    simp only [dv]
+    apply Finset.union_subset_union_right
+    exact h
+  }
+
+theorem Ctx.closeSubtermsOver_min (Γ : Ctx) (σ : Tm.BSubst) (a : Tm)
+  : Γ.closeSubtermsOver σ a ⊆ Ctx.nil.closeSubtermsOver σ a
+  := closeSubtermsOver_anti _ _ _ _ (by simp [dv])
+
+def Ctx.tys : Ctx → Finset Tm
+  | .nil => ∅
+  | .cons Γ _ A => { A } ∪ Γ.tys
+
+def Ctx.subterms (Γ : Ctx) : Set Tm := ⋃ A ∈ Γ.tys, Γ.closeSubtermsOver 1 A
+
+def Ctx.strictSubtermsOver (Γ : Ctx) (a : Tm) : Set Tm := (Γ.closeSubtermsOver 1 a) \ {a}
+
+@[simp]
+theorem Ctx.mem_closeSubtermsOver1 (Γ : Ctx) (a : Tm)
+  : a ∈ Γ.closeSubtermsOver 1 a := by cases a <;> simp
+
+theorem Ctx.closeSubtermsOver1_strict (Γ : Ctx) (a : Tm)
+  : Γ.closeSubtermsOver 1 a = {a} ∪ Γ.strictSubtermsOver a
+  := by simp [strictSubtermsOver]
+
+@[simp]
+theorem Ctx.strictSubtermsOver_fv (Γ : Ctx) (x : ℕ)
+  : Γ.strictSubtermsOver (.fv x) = ∅
+  := by simp [strictSubtermsOver]
+
+@[simp]
+theorem Ctx.strictSubtermsOver_bv (Γ : Ctx) (i : ℕ)
+  : Γ.strictSubtermsOver (.bv i) = ∅
+  := by simp [strictSubtermsOver]
+
+@[simp]
+theorem Ctx.strictSubtermsOver_univ (Γ : Ctx) (ℓ : ℕ)
+  : Γ.strictSubtermsOver (.univ ℓ) = ∅
+  := by simp [strictSubtermsOver]
+
+@[simp]
+theorem Ctx.strictSubtermsOver_unit (Γ : Ctx) (ℓ : ℕ)
+  : Γ.strictSubtermsOver (.unit ℓ) = ∅
+  := by simp [strictSubtermsOver]
+
+@[simp]
+theorem Ctx.strictSubtermsOver_nil (Γ : Ctx) (ℓ : ℕ)
+  : Γ.strictSubtermsOver (.nil ℓ) = ∅
+  := by simp [strictSubtermsOver]
+
+@[simp]
+theorem Ctx.strictSubtermsOver_empty (Γ : Ctx) (ℓ : ℕ)
+  : Γ.strictSubtermsOver (.empty ℓ) = ∅
+  := by simp [strictSubtermsOver]
+
+-- theorem Ctx.strictSubtermsOver_eqn (Γ : Ctx) (A a b : Tm)
+--   : Γ.strictSubtermsOver (.eqn A a b)
+--   = {A} ∪ {a} ∪ {b} ∪ Γ.strictSubtermsOver A ∪ Γ.strictSubtermsOver a ∪ Γ.strictSubtermsOver b
+--   := by
+--   simp only [strictSubtermsOver, closeSubtermsOver1_eqn]
+--   rw [Set.union_assoc, Set.union_assoc, Set.union_comm, Set.diff_union_self]
+--   simp only [Set.distrib_]
+
+@[simp]
+theorem Ctx.strictSubtermsOver_nats (Γ : Ctx)
+  : Γ.strictSubtermsOver .nats = ∅
+  := by simp [strictSubtermsOver]
+
+
+theorem Ctx.strictSubtermsOverIndHelper (Γ : Ctx)
+  (motive : Tm → Prop)
+  (h : ∀ a, motive a ∧ ∀ b ∈ Γ.strictSubtermsOver a, motive b)
+  : ∀ a, motive a
+  := fun a => (h a).1
+
+-- theorem Ctx.strictSubtermsOverInd (Γ : Ctx)
+--   (motive : Tm → Prop)
+--   (h : (∀ a, (∀ b ∈ Γ.strictSubtermsOver a, motive b) → motive a))
+--   : ∀ a, motive a
+--   := by
+--   apply Ctx.strictSubtermsOverIndHelper .nil
+--   intro a
+--   generalize hb: a = b
+--   induction b generalizing a with
+--   | fv =>
+--     have ha := h a
+--     simp [hb, strictSubtermsOver] at ha
+--     simp [ha]
+--   | pi =>
+--     have ha := h a
+--     cases hb
+--     simp at *
+--     sorry
+--   | _ => sorry
+
+-- def Ctx.strictSubterms (Γ : Ctx) (a : Tm) : Set Tm := Γ.subterms ∪ Γ.strictSubtermsOver a
+
+-- theorem Ctx.closeSubtermsInd
+--   (motive : Ctx → Tm → Prop)
+--   (h : (∀ Γ a, (∀ b ∈ Γ.strictSubterms a, motive Γ b) → motive Γ a))
+--   : ∀ Γ a, motive Γ a
+--   := by
+--   intro Γ a
+--   revert Γ
+--   induction a using closeSubtermsOverInd .nil with
+--   | h a I =>
+--     sorry
+
+inductive Ctx.StrictSubterms : Ctx → Tm → Set Tm
+  | cons {Γ : Ctx} {x} {a A  : Tm} : (Γ.cons x A).StrictSubterms a A
+  | sub_cons {Γ : Ctx} {x} {A s a : Tm} : Γ.StrictSubterms A s → (Γ.cons x A).StrictSubterms a s
+  | eqn_ty {Γ : Ctx} {A a b : Tm} : Γ.StrictSubterms (.eqn A a b) A
+  | sub_eqn_ty {Γ : Ctx} {A a b s : Tm} : Γ.StrictSubterms A s → Γ.StrictSubterms (.eqn A a b) s
+  | eqn_lhs {Γ : Ctx} {A a b : Tm} : Γ.StrictSubterms (.eqn A a b) a
+  | sub_eqn_lhs {Γ : Ctx} {A a b s : Tm} : Γ.StrictSubterms a s → Γ.StrictSubterms (.eqn A a b) s
+  | eqn_rhs {Γ : Ctx} {A a b : Tm} : Γ.StrictSubterms (.eqn A a b) b
+  | sub_eqn_rhs {Γ : Ctx} {A a b s : Tm} : Γ.StrictSubterms b s → Γ.StrictSubterms (.eqn A a b) s
+  | pi_ty {Γ : Ctx} {A B : Tm} : Γ.StrictSubterms (.pi A B) A
+  | sub_pi_ty {Γ : Ctx} {A B s : Tm} : Γ.StrictSubterms A s → Γ.StrictSubterms (.pi A B) s
+  | pi_body {Γ : Ctx} {x : ℕ} {A B : Tm} : x ∉ Γ.dv → Γ.StrictSubterms (.pi A B) (B.bs0 (.fv x))
+  | sub_pi_body {Γ : Ctx} {x : ℕ} {A B s : Tm}
+    : x ∉ Γ.dv → (Γ.cons x A).StrictSubterms (B.bs0 (.fv x)) s → Γ.StrictSubterms (.pi A B) s
+  | abs_ty {Γ : Ctx} {A B b : Tm} : Γ.StrictSubterms (.abs A B b) A
+  | sub_abs_ty {Γ : Ctx} {A B b s : Tm} : Γ.StrictSubterms A s → Γ.StrictSubterms (.abs A B b) s
+  | abs_res {Γ : Ctx} {x : ℕ} {A B b : Tm}
+    : x ∉ Γ.dv → Γ.StrictSubterms (.abs A B b) (B.bs0 (.fv x))
+  | sub_abs_res {Γ : Ctx} {x : ℕ} {A B b s : Tm}
+    : x ∉ Γ.dv → (Γ.cons x A).StrictSubterms (B.bs0 (.fv x)) s → Γ.StrictSubterms (.abs A B b) s
+  | abs_body {Γ : Ctx} {x : ℕ} {A B b : Tm}
+    : x ∉ Γ.dv → Γ.StrictSubterms (.abs A B b) (b.bs0 (.fv x))
+  | sub_abs_body {Γ : Ctx} {x : ℕ} {A B b s : Tm}
+    : x ∉ Γ.dv → (Γ.cons x A).StrictSubterms (b.bs0 (.fv x)) s → Γ.StrictSubterms (.abs A B b) s
+  | app_ty {Γ : Ctx} {A B f a : Tm} : Γ.StrictSubterms (.app A B f a) A
+  | sub_app_ty {Γ : Ctx} {A B f a s : Tm}
+    : Γ.StrictSubterms A s → Γ.StrictSubterms (.app A B f a) s
+  | app_res {Γ : Ctx} {x : ℕ} {A B f a : Tm}
+    : x ∉ Γ.dv → Γ.StrictSubterms (.app A B f a) (B.bs0 (.fv x))
+  | sub_app_res {Γ : Ctx} {x : ℕ} {A B f a s : Tm}
+    : x ∉ Γ.dv → (Γ.cons x A).StrictSubterms (B.bs0 (.fv x)) s → Γ.StrictSubterms (.app A B f a) s
+  | app_f {Γ : Ctx} {A B f a : Tm} : Γ.StrictSubterms (.app A B f a) f
+  | sub_app_f {Γ : Ctx} {A B f a s : Tm}
+    : Γ.StrictSubterms f s → Γ.StrictSubterms (.app A B f a) s
+  | app_a {Γ : Ctx} {A B f a : Tm} : Γ.StrictSubterms (.app A B f a) a
+  | sub_app_a {Γ : Ctx} {A B f a s : Tm}
+    : Γ.StrictSubterms a s → Γ.StrictSubterms (.app A B f a) s
+  | sigma_ty {Γ : Ctx} {A B : Tm} : Γ.StrictSubterms (.sigma A B) A
+  | sub_sigma_ty {Γ : Ctx} {A B s : Tm} : Γ.StrictSubterms A s → Γ.StrictSubterms (.sigma A B) s
+  | sigma_body {Γ : Ctx} {x : ℕ} {A B : Tm}
+    : x ∉ Γ.dv → Γ.StrictSubterms (.sigma A B) (B.bs0 (.fv x))
+  | sub_sigma_body {Γ : Ctx} {x : ℕ} {A B s : Tm}
+    : x ∉ Γ.dv → (Γ.cons x A).StrictSubterms (B.bs0 (.fv x)) s → Γ.StrictSubterms (.sigma A B) s
+  | pair_ty {Γ : Ctx} {A B a b : Tm} : Γ.StrictSubterms (.pair A B a b) A
+  | sub_pair_ty {Γ : Ctx} {A B a b s : Tm}
+    : Γ.StrictSubterms A s → Γ.StrictSubterms (.pair A B a b) s
+  | pair_res {Γ : Ctx} {x : ℕ} {A B a b : Tm}
+    : x ∉ Γ.dv → Γ.StrictSubterms (.pair A B a b) (B.bs0 (.fv x))
+  | sub_pair_res {Γ : Ctx} {x : ℕ} {A B a b s : Tm}
+    : x ∉ Γ.dv → (Γ.cons x A).StrictSubterms (B.bs0 (.fv x)) s → Γ.StrictSubterms (.pair A B a b) s
+  | pair_a {Γ : Ctx} {A B a b : Tm} : Γ.StrictSubterms (.pair A B a b) a
+  | sub_pair_a {Γ : Ctx} {A B a b s : Tm}
+    : Γ.StrictSubterms a s → Γ.StrictSubterms (.pair A B a b) s
+  | pair_b {Γ : Ctx} {A B a b : Tm} : Γ.StrictSubterms (.pair A B a b) b
+  | sub_pair_b {Γ : Ctx} {A B a b s : Tm}
+    : Γ.StrictSubterms b s → Γ.StrictSubterms (.pair A B a b) s
+  | fst_ty {Γ : Ctx} {A B a : Tm} : Γ.StrictSubterms (.fst A B a) A
+  | sub_fst_ty {Γ : Ctx} {A B a s : Tm}
+    : Γ.StrictSubterms A s → Γ.StrictSubterms (.fst A B a) s
+  | fst_body {Γ : Ctx} {x : ℕ} {A B a : Tm}
+    : x ∉ Γ.dv → Γ.StrictSubterms (.fst A B a) (B.bs0 (.fv x))
+  | sub_fst_body {Γ : Ctx} {x : ℕ} {A B a s : Tm}
+    : x ∉ Γ.dv → (Γ.cons x A).StrictSubterms (B.bs0 (.fv x)) s → Γ.StrictSubterms (.fst A B a) s
+  | fst_a {Γ : Ctx} {A B a : Tm} : Γ.StrictSubterms (.fst A B a) a
+  | sub_fst_a {Γ : Ctx} {A B a s : Tm}
+    : Γ.StrictSubterms a s → Γ.StrictSubterms (.fst A B a) s
+  | snd_ty {Γ : Ctx} {A B a : Tm} : Γ.StrictSubterms (.snd A B a) A
+  | sub_snd_ty {Γ : Ctx} {A B a s : Tm}
+    : Γ.StrictSubterms A s → Γ.StrictSubterms (.snd A B a) s
+  | snd_body {Γ : Ctx} {x : ℕ} {A B a : Tm}
+    : x ∉ Γ.dv → Γ.StrictSubterms (.snd A B a) (B.bs0 (.fv x))
+  | sub_snd_body {Γ : Ctx} {x : ℕ} {A B a s : Tm}
+    : x ∉ Γ.dv → (Γ.cons x A).StrictSubterms (B.bs0 (.fv x)) s → Γ.StrictSubterms (.snd A B a) s
+  | snd_a {Γ : Ctx} {A B a : Tm} : Γ.StrictSubterms (.snd A B a) a
+  | sub_snd_a {Γ : Ctx} {A B a s : Tm}
+    : Γ.StrictSubterms a s → Γ.StrictSubterms (.snd A B a) s
+  | dite_ty {Γ : Ctx} {φ A a b : Tm} : Γ.StrictSubterms (.dite φ A a b) φ
+  | sub_dite_ty {Γ : Ctx} {φ A a b s : Tm}
+    : Γ.StrictSubterms φ s → Γ.StrictSubterms (.dite φ A a b) s
+  | dite_a {Γ : Ctx} {φ A a b : Tm} : Γ.StrictSubterms (.dite φ A a b) A
+  | sub_dite_a {Γ : Ctx} {φ A a b s : Tm}
+    : Γ.StrictSubterms A s → Γ.StrictSubterms (.dite φ A a b) s
+  | dite_b {Γ : Ctx} {φ A a b : Tm} : Γ.StrictSubterms (.dite φ A a b) A
+  | sub_dite_b {Γ : Ctx} {φ A a b s : Tm}
+    : Γ.StrictSubterms A s → Γ.StrictSubterms (.dite φ A a b) s
+  | dite_a_true {Γ : Ctx} {φ A a b : Tm}
+    : Γ.StrictSubterms (.dite φ A a b) a
+  | sub_dite_a_true {Γ : Ctx} {φ A a b s : Tm}
+    : Γ.StrictSubterms a s → Γ.StrictSubterms (.dite φ A a b) s
+  | dite_b_false {Γ : Ctx} {φ A a b : Tm}
+    : Γ.StrictSubterms (.dite φ A a b) b
+  | sub_dite_b_false {Γ : Ctx} {φ A a b s : Tm}
+    : Γ.StrictSubterms b s → Γ.StrictSubterms (.dite φ A a b) s
+  | trunc {Γ : Ctx} {A : Tm} : Γ.StrictSubterms (.trunc A) A
+  | sub_trunc {Γ : Ctx} {A s : Tm}
+    : Γ.StrictSubterms A s → Γ.StrictSubterms (.trunc A) s
+  | choose_ty {Γ : Ctx} {A φ : Tm} : Γ.StrictSubterms (.choose A φ) A
+  | sub_choose_ty {Γ : Ctx} {A φ s : Tm}
+    : Γ.StrictSubterms A s → Γ.StrictSubterms (.choose A φ) s
+  | choose_body {Γ : Ctx} {x : ℕ} {A φ : Tm}
+    : x ∉ Γ.dv → Γ.StrictSubterms (.choose A φ) (φ.bs0 (.fv x))
+  | sub_choose_body {Γ : Ctx} {x : ℕ} {A φ s : Tm}
+    : x ∉ Γ.dv → (Γ.cons x A).StrictSubterms (φ.bs0 (.fv x)) s
+    → Γ.StrictSubterms (.choose A φ) s
+  | natrec_ty {Γ : Ctx} {C n z s : Tm} : Γ.StrictSubterms (.natrec C n z s) C
+  | sub_natrec_ty {Γ : Ctx} {C n z s : Tm}
+    : Γ.StrictSubterms C s → Γ.StrictSubterms (.natrec C n z s) s
+  | natrec_n {Γ : Ctx} {C n z s : Tm} : Γ.StrictSubterms (.natrec C n z s) n
+  | sub_natrec_n {Γ : Ctx} {C n z s : Tm}
+    : Γ.StrictSubterms n s → Γ.StrictSubterms (.natrec C n z s) s
+  | natrec_z {Γ : Ctx} {C n z s : Tm} : Γ.StrictSubterms (.natrec C n z s) z
+  | sub_natrec_z {Γ : Ctx} {C n z s : Tm}
+    : Γ.StrictSubterms z s → Γ.StrictSubterms (.natrec C n z s) s
+  | natrec_s {Γ : Ctx} {x : ℕ} {C n z s : Tm}
+    : x ∉ Γ.dv → Γ.StrictSubterms (.natrec C n z s) (s.bs0 (.fv x))
+  | sub_natrec_s {Γ : Ctx} {x : ℕ} {C n z s : Tm}
+    : x ∉ Γ.dv → (Γ.cons x C).StrictSubterms (s.bs0 (.fv x)) s
+    → Γ.StrictSubterms (.natrec C n z s) s
